Dafny opaque all invariants (#2914)
* Added opaque for performance experiment.

* Progress with opaque-ing on reducing verifier timeouts

* Progress in preformance inprovements.

* Second Invarinat proof.

* Refactor for easier case analysis for the honest replica actions.

* Case split for that Hones Replica steps preserve each predicate of the Invariant.

* Refactor EveryPrepareClientOpMatchesRecordedPrePrepare predicate.

We refactor the predicate, which is part of the Inv to not bind the
state of the network to the internal state of the replicas.
Added reasoning in the case analysis for preserving
EveryCommitIsSupportedByPreviouslySentPrepares.

* Clenup CommitMsgStability in progress.

* Code restructuring to reason about each component of the invariant separately.

* Finalized proof refactoring.

docs/sbft-formal-model/proof.dfy
@@ -36,7 +36,7 @@ module Proof {
   }
 
   // Here's a predicate that will be very useful in constructing invariant conjuncts.
-  predicate RecordedPrePreparesRecvdCameFromNetwork(c:Constants, v:Variables) {
+  predicate {:opaque} RecordedPrePreparesRecvdCameFromNetwork(c:Constants, v:Variables) {
     && v.WF(c)
     && (forall replicaIdx, seqID | 
               && IsHonestReplica(c, replicaIdx)
@@ -62,14 +62,14 @@ module Proof {
                     && msg.payload.seqID == seqID)) // The key we stored matches what is in the msg
   }
 
-  predicate RecordedPreparesInAllHostsRecvdCameFromNetwork(c:Constants, v:Variables) {
+  predicate {:opaque} RecordedPreparesInAllHostsRecvdCameFromNetwork(c:Constants, v:Variables) {
     && v.WF(c)
     && (forall observer | 
             && IsHonestReplica(c, observer)
                 :: RecordedPreparesRecvdCameFromNetwork(c, v, observer))
   }
 
-  predicate EveryCommitMsgIsSupportedByAQuorumOfPrepares(c:Constants, v:Variables) {
+  predicate {:opaque} EveryCommitMsgIsSupportedByAQuorumOfPrepares(c:Constants, v:Variables) {
     && v.WF(c)
     && (forall commitMsg | && commitMsg in v.network.sentMsgs 
                            && commitMsg.payload.Commit? 
@@ -82,7 +82,7 @@ module Proof {
   // with a Prepare message only for it. The lock on Prepare is meant to highlight the fact that
   // even though a replica can send multiple times a Prepare message for a given Sequence ID for
   // a given View, this message will not change unless a View Change happens.
-  predicate HonestReplicasLockOnPrepareForGivenView(c: Constants, v:Variables)
+  predicate {:opaque} HonestReplicasLockOnPrepareForGivenView(c: Constants, v:Variables)
   {
     && (forall msg1, msg2 {:trigger msg1.payload.Prepare?, msg2.payload.Prepare?} | 
         && msg1 in v.network.sentMsgs 
@@ -125,7 +125,7 @@ module Proof {
         :: msg1.payload.operationWrapper == msg2.payload.operationWrapper)
   }
 
-  predicate RecordedPreparesHaveValidSenderID(c:Constants, v:Variables) {
+  predicate {:opaque} RecordedPreparesHaveValidSenderID(c:Constants, v:Variables) {
     && v.WF(c)
     && (forall replicaIdx, seqID, sender |
           && IsHonestReplica(c, replicaIdx)
@@ -133,11 +133,10 @@ module Proof {
           && seqID in prepareMap
           && sender in prepareMap[seqID]
           :: && v.hosts[replicaIdx].replicaVariables.workingWindow.preparesRcvd[seqID][sender].sender == sender
-             && c.clusterConfig.IsReplica(sender)
         )
   }
 
-  predicate RecordedPreparesClientOpsMatchPrePrepare(c:Constants, v:Variables) {
+  predicate {:opaque} RecordedPreparesClientOpsMatchPrePrepare(c:Constants, v:Variables) {
     && v.WF(c)
     && (forall replicaIdx, seqID, sender |
           && IsHonestReplica(c, replicaIdx)
@@ -173,16 +172,7 @@ module Proof {
                                          commitMsg.payload.seqID))
   }
 
-  predicate {:opaque} EveryCommitIsSupportedByPreviouslySentPrepares(c:Constants, v:Variables) {
-    && v.WF(c)
-    && (forall commitMsg | && commitMsg in v.network.sentMsgs
-                           && commitMsg.payload.Commit?
-                           && IsHonestReplica(c, commitMsg.sender)
-          :: QuorumOfPreparesInNetwork(c, v, commitMsg.payload.view, 
-                                       commitMsg.payload.seqID, commitMsg.payload.operationWrapper))
-  }
-
-  predicate EverySentIntraViewMsgIsInWorkingWindowOrBefore(c:Constants, v:Variables) {
+  predicate {:opaque} EverySentIntraViewMsgIsInWorkingWindowOrBefore(c:Constants, v:Variables) {
     && v.WF(c)
     && (forall msg | && msg in v.network.sentMsgs
                            && msg.payload.IsIntraViewMsg()
@@ -192,7 +182,7 @@ module Proof {
              && msg.payload.seqID < replicaVariables.workingWindow.lastStableCheckpoint + replicaConstants.clusterConfig.workingWindowSize)
   }
 
-  predicate EverySentIntraViewMsgIsForAViewLessOrEqualToSenderView(c:Constants, v:Variables) {
+  predicate {:opaque} EverySentIntraViewMsgIsForAViewLessOrEqualToSenderView(c:Constants, v:Variables) {
     && v.WF(c)
     && (forall msg | && msg in v.network.sentMsgs
                            && msg.payload.IsIntraViewMsg()
@@ -219,20 +209,21 @@ module Proof {
 
   predicate {:opaque} EveryPrepareClientOpMatchesRecordedPrePrepare(c:Constants, v:Variables) {
     && v.WF(c)
-    && (forall prepareMsg | && prepareMsg in v.network.sentMsgs
-                           && prepareMsg.payload.Prepare?
-                           && IsHonestReplica(c, prepareMsg.sender)
-                           && var replicaVariables := v.hosts[prepareMsg.sender].replicaVariables;
-                           && var replicaConstants := c.hosts[prepareMsg.sender].replicaConstants;
-                           && prepareMsg.payload.seqID in replicaVariables.workingWindow.getActiveSequenceIDs(replicaConstants)
-                           && prepareMsg.payload.view == replicaVariables.view
+    && (forall prepareMsg | 
+                      && prepareMsg in v.network.sentMsgs
+                      && prepareMsg.payload.Prepare?
+                      && IsHonestReplica(c, prepareMsg.sender)
+                      && var replicaVariables := v.hosts[prepareMsg.sender].replicaVariables;
+                      && var replicaConstants := c.hosts[prepareMsg.sender].replicaConstants;
+                      && prepareMsg.payload.seqID in replicaVariables.workingWindow.getActiveSequenceIDs(replicaConstants)
+                      && prepareMsg.payload.view == replicaVariables.view
           :: && var recordedPrePrepare := 
                 v.hosts[prepareMsg.sender].replicaVariables.workingWindow.prePreparesRcvd[prepareMsg.payload.seqID];
              && recordedPrePrepare.Some?
              && prepareMsg.payload.operationWrapper == recordedPrePrepare.value.payload.operationWrapper)
   }
 
-  predicate RecordedPreparesMatchHostView(c:Constants, v:Variables) {
+  predicate {:opaque} RecordedPreparesMatchHostView(c:Constants, v:Variables) {
     && v.WF(c)
     && (forall observer, seqID, sender | 
                            && IsHonestReplica(c, observer)
@@ -260,7 +251,7 @@ module Proof {
                         == prepare.payload.operationWrapper)
   }
 
-  predicate RecordedCheckpointsRecvdCameFromNetwork(c:Constants, v:Variables) {
+  predicate {:opaque} RecordedCheckpointsRecvdCameFromNetwork(c:Constants, v:Variables) {
     && v.WF(c)
     && (forall replicaIdx, checkpointMsg | 
               && IsHonestReplica(c, replicaIdx)
@@ -283,7 +274,7 @@ module Proof {
   //                                       :: prePrepare1 == prePrepare2)
   // }
 
-  predicate AllReplicasLiteInv (c: Constants, v:Variables) {
+  predicate {:opaque} AllReplicasLiteInv (c: Constants, v:Variables) {
     && v.WF(c)
     && (forall replicaIdx | 0 <= replicaIdx < |c.hosts| && c.clusterConfig.IsHonestReplica(replicaIdx)
                             :: Replica.LiteInv(c.hosts[replicaIdx].replicaConstants, v.hosts[replicaIdx].replicaVariables))
@@ -301,7 +292,6 @@ module Proof {
     && EveryCommitMsgIsSupportedByAQuorumOfPrepares(c, v)
     && RecordedPreparesClientOpsMatchPrePrepare(c, v)
     && RecordedCommitsClientOpsMatchPrePrepare(c, v)
-    && EveryCommitIsSupportedByPreviouslySentPrepares(c, v)
     && EverySentIntraViewMsgIsInWorkingWindowOrBefore(c, v)
     && EverySentIntraViewMsgIsForAViewLessOrEqualToSenderView(c, v)
     && EveryPrepareClientOpMatchesRecordedPrePrepare(c, v)
@@ -348,6 +338,12 @@ module Proof {
     requires IsHonestReplica(c, msg2.sender)
     ensures msg1.payload.operationWrapper == msg2.payload.operationWrapper
   {
+    reveal_RecordedPreparesInAllHostsRecvdCameFromNetwork();
+    reveal_RecordedPreparesMatchHostView();
+    reveal_RecordedPreparesClientOpsMatchPrePrepare();
+    reveal_HonestReplicasLockOnPrepareForGivenView();
+    reveal_EveryCommitMsgIsSupportedByAQuorumOfPrepares();
+
     var prepares1 := sentPreparesForSeqID(c, v, msg1.payload.view, msg1.payload.seqID, msg1.payload.operationWrapper);
     var senders1 := Messages.sendersOf(prepares1);
     assert |senders1| >= c.clusterConfig.AgreementQuorum();
@@ -356,6 +352,8 @@ module Proof {
     var h_v := v.hosts[step.id].replicaVariables;
     var h_v' := v'.hosts[step.id].replicaVariables;
     var h_step :| Replica.NextStep(h_c, h_v, h_v', step.msgOps, h_step);
+
+    h_v.workingWindow.reveal_Shift();
 
     var senders2 := h_v.workingWindow.preparesRcvd[h_step.seqID].Keys;
     assert |senders2| >= c.clusterConfig.AgreementQuorum();
@@ -453,9 +451,226 @@ module Proof {
       }
   }
 
-  lemma ProofCommitMsgsFromHonestSendersAgree(c: Constants, v:Variables, v':Variables, step:Step)
+  predicate HonestReplicaStepTaken(c: Constants, v:Variables, v':Variables, step:Step, h_v:Replica.Variables, h_step:Replica.Step)
+  {
+    && v.WF(c)
+    && v'.WF(c)
+    && NextStep(c, v, v', step)
+    && IsHonestReplica(c, step.id)
+    && var h_c := c.hosts[step.id].replicaConstants;
+    && h_v == v.hosts[step.id].replicaVariables
+    && var h_v' := v'.hosts[step.id].replicaVariables;
+    && Replica.NextStep(h_c, h_v, h_v', step.msgOps, h_step)
+  }
+
+  lemma HonestPreservesAllReplicasLiteInv(c: Constants, v:Variables, v':Variables, step:Step, h_v:Replica.Variables, h_step:Replica.Step)
+    requires Inv(c, v)
+    requires HonestReplicaStepTaken(c, v, v', step, h_v, h_step)
+    ensures AllReplicasLiteInv(c, v')
+  {
+    reveal_AllReplicasLiteInv();
+  }
+
+  lemma HonestPreservesRecordedPreparesHaveValidSenderID(c: Constants, v:Variables, v':Variables, step:Step, h_v:Replica.Variables, h_step:Replica.Step)
+    requires Inv(c, v)
+    requires HonestReplicaStepTaken(c, v, v', step, h_v, h_step)
+    ensures RecordedPreparesHaveValidSenderID(c, v')
+  {
+    reveal_RecordedPreparesHaveValidSenderID();
+
+    if (h_step.AdvanceWorkingWindowStep?) {
+      h_v.workingWindow.reveal_Shift();
+    } else if(h_step.PerformStateTransferStep?) {
+      h_v.workingWindow.reveal_Shift();
+    }
+  }
+
+  lemma HonestPreservesRecordedPrePreparesRecvdCameFromNetwork(c: Constants, v:Variables, v':Variables, step:Step, h_v:Replica.Variables, h_step:Replica.Step)
+    requires Inv(c, v)
+    requires HonestReplicaStepTaken(c, v, v', step, h_v, h_step)
+    ensures RecordedPrePreparesRecvdCameFromNetwork(c, v')
+  {
+    reveal_RecordedPrePreparesRecvdCameFromNetwork();
+
+    if (h_step.AdvanceWorkingWindowStep?) {
+      h_v.workingWindow.reveal_Shift();
+    } else if(h_step.PerformStateTransferStep?) {
+      h_v.workingWindow.reveal_Shift();
+    }
+  }
+
+  lemma HonestPreservesRecordedPreparesInAllHostsRecvdCameFromNetwork(c: Constants, v:Variables, v':Variables, step:Step, h_v:Replica.Variables, h_step:Replica.Step)
+    requires Inv(c, v)
+    requires HonestReplicaStepTaken(c, v, v', step, h_v, h_step)
+    ensures RecordedPreparesInAllHostsRecvdCameFromNetwork(c, v')
+  {
+    reveal_RecordedPreparesInAllHostsRecvdCameFromNetwork();
+
+    if (h_step.AdvanceWorkingWindowStep?) {
+      h_v.workingWindow.reveal_Shift();
+    } else if(h_step.PerformStateTransferStep?) {
+      h_v.workingWindow.reveal_Shift();
+    }
+  }
+
+  lemma HonestPreservesRecordedPreparesMatchHostView(c: Constants, v:Variables, v':Variables, step:Step, h_v:Replica.Variables, h_step:Replica.Step)
+    requires Inv(c, v)
+    requires HonestReplicaStepTaken(c, v, v', step, h_v, h_step)
+    ensures RecordedPreparesMatchHostView(c, v')
+  {
+    reveal_RecordedPreparesMatchHostView();
+
+    if (h_step.AdvanceWorkingWindowStep?) {
+      h_v.workingWindow.reveal_Shift();
+    } else if(h_step.PerformStateTransferStep?) {
+      h_v.workingWindow.reveal_Shift();
+    }
+  }
+
+  lemma AlwaysPreservesEveryCommitMsgIsSupportedByAQuorumOfPrepares(c: Constants, v:Variables, v':Variables, step:Step)
     requires Inv(c, v)
     requires NextStep(c, v, v', step)
+    ensures EveryCommitMsgIsSupportedByAQuorumOfPrepares(c, v')
+  {
+    reveal_EveryCommitMsgIsSupportedByAQuorumOfPrepares();
+    // A proof of EveryCommitMsgIsSupportedByAQuorumOfPrepares,
+    // by selecting an arbitrary commitMsg instance
+    forall commitMsg | && commitMsg in v'.network.sentMsgs 
+                       && commitMsg.payload.Commit?
+                       && IsHonestReplica(c, commitMsg.sender) ensures 
+      QuorumOfPreparesInNetwork(c, v', commitMsg.payload.view, commitMsg.payload.seqID, commitMsg.payload.operationWrapper) {
+      if(commitMsg in v.network.sentMsgs) { // the commitMsg has been sent in a previous step
+        // In this case, the proof is trivial - we just need to "teach" Dafny about subset cardinality
+        var senders := Messages.sendersOf(sentPreparesForSeqID(c, v, commitMsg.payload.view, 
+                                                      commitMsg.payload.seqID, commitMsg.payload.operationWrapper));
+        var senders' := Messages.sendersOf(sentPreparesForSeqID(c, v', commitMsg.payload.view,
+                                                      commitMsg.payload.seqID, commitMsg.payload.operationWrapper));
+        Library.SubsetCardinality(senders, senders');
+      } else { // the commitMsg is being sent in the current step
+        reveal_RecordedPreparesInAllHostsRecvdCameFromNetwork();
+        reveal_RecordedPreparesMatchHostView();
+        reveal_RecordedPreparesClientOpsMatchPrePrepare();
+        var prepares := sentPreparesForSeqID(c, v, commitMsg.payload.view,
+                                             commitMsg.payload.seqID, commitMsg.payload.operationWrapper);
+        var prepares' := sentPreparesForSeqID(c, v', commitMsg.payload.view, 
+                                             commitMsg.payload.seqID, commitMsg.payload.operationWrapper);
+        assert prepares == prepares'; // Trigger (hint) - sending a commitMsg does not affect the set of prepares
+        
+        // Prove that the prepares in the working window are a subset of the prepares in the network:
+        var prepareSendersFromNetwork := Messages.sendersOf(prepares);
+        var h_v := v.hosts[step.id];
+        var prepareSendersInWorkingWindow := h_v.replicaVariables.workingWindow.preparesRcvd[commitMsg.payload.seqID].Keys;
+        assert (forall sender | sender in prepareSendersInWorkingWindow 
+                              :: && var msg := h_v.replicaVariables.workingWindow.preparesRcvd[commitMsg.payload.seqID][sender];
+                                 && msg in v.network.sentMsgs);
+        assert (forall sender | sender in prepareSendersInWorkingWindow 
+                              :: sender in prepareSendersFromNetwork); //Trigger for subset operator
+        Library.SubsetCardinality(prepareSendersInWorkingWindow, prepareSendersFromNetwork);
+      }
+    }
+  }
+
+  lemma HonestPreservesRecordedPreparesClientOpsMatchPrePrepare(c: Constants, v:Variables, v':Variables, step:Step, h_v:Replica.Variables, h_step:Replica.Step)
+    requires Inv(c, v)
+    requires HonestReplicaStepTaken(c, v, v', step, h_v, h_step)
+    ensures RecordedPreparesClientOpsMatchPrePrepare(c, v')
+  {
+    reveal_RecordedPreparesClientOpsMatchPrePrepare();
+
+    if (h_step.AdvanceWorkingWindowStep?) {
+      h_v.workingWindow.reveal_Shift();
+    } else if(h_step.PerformStateTransferStep?) {
+      h_v.workingWindow.reveal_Shift();
+    }
+  }
+
+  lemma HonestPreservesRecordedCommitsClientOpsMatchPrePrepare(c: Constants, v:Variables, v':Variables, step:Step, h_v:Replica.Variables, h_step:Replica.Step)
+    requires Inv(c, v)
+    requires HonestReplicaStepTaken(c, v, v', step, h_v, h_step)
+    ensures RecordedCommitsClientOpsMatchPrePrepare(c, v')
+  {
+    reveal_RecordedCommitsClientOpsMatchPrePrepare();
+
+    if (h_step.AdvanceWorkingWindowStep?) {
+      h_v.workingWindow.reveal_Shift();
+    } else if(h_step.PerformStateTransferStep?) {
+      h_v.workingWindow.reveal_Shift();
+    }
+  }
+
+  lemma CountPrepareMessages(proofSet:Replica.PrepareProofSet)
+    requires forall sender | sender in proofSet.Keys :: proofSet[sender].sender == sender
+    ensures |proofSet.Values| == |proofSet.Keys|
+  {
+    if |proofSet.Keys| > 0 {
+      var element :| element in proofSet.Keys;
+      var subMap := MapRemoveOne(proofSet, element);
+      CountPrepareMessages(subMap);
+      assert proofSet.Values == subMap.Values + {proofSet[element]};
+      assert proofSet.Keys == subMap.Keys + {element};
+    }
+  }
+
+  lemma HonestPreservesEveryPrepareClientOpMatchesRecordedPrePrepare(c: Constants, v:Variables, v':Variables, step:Step, h_v:Replica.Variables, h_step:Replica.Step)
+    requires Inv(c, v)
+    requires HonestReplicaStepTaken(c, v, v', step, h_v, h_step)
+    ensures EveryPrepareClientOpMatchesRecordedPrePrepare(c, v')
+
+  {
+    reveal_EveryPrepareClientOpMatchesRecordedPrePrepare();
+    reveal_EverySentIntraViewMsgIsInWorkingWindowOrBefore();
+    reveal_EverySentIntraViewMsgIsForAViewLessOrEqualToSenderView();
+    h_v.workingWindow.reveal_Shift();
+  }
+
+  lemma HonestPreservesEverySentIntraViewMsgIsInWorkingWindowOrBefore(c: Constants, v:Variables, v':Variables, step:Step, h_v:Replica.Variables, h_step:Replica.Step)
+    requires Inv(c, v)
+    requires HonestReplicaStepTaken(c, v, v', step, h_v, h_step)
+    ensures EverySentIntraViewMsgIsInWorkingWindowOrBefore(c, v')
+  {
+    reveal_EverySentIntraViewMsgIsInWorkingWindowOrBefore();
+  }
+
+  lemma HonestPreservesEverySentIntraViewMsgIsForAViewLessOrEqualToSenderView(c: Constants, v:Variables, v':Variables, step:Step, h_v:Replica.Variables, h_step:Replica.Step)
+    requires Inv(c, v)
+    requires HonestReplicaStepTaken(c, v, v', step, h_v, h_step)
+    ensures EverySentIntraViewMsgIsForAViewLessOrEqualToSenderView(c, v')
+  {
+    reveal_EverySentIntraViewMsgIsForAViewLessOrEqualToSenderView();
+  }
+
+  lemma HonestPreservesEveryCommitClientOpMatchesRecordedPrePrepare(c: Constants, v:Variables, v':Variables, step:Step, h_v:Replica.Variables, h_step:Replica.Step)
+    requires Inv(c, v)
+    requires HonestReplicaStepTaken(c, v, v', step, h_v, h_step)
+    ensures EveryCommitClientOpMatchesRecordedPrePrepare(c, v')
+  {
+    reveal_EverySentIntraViewMsgIsInWorkingWindowOrBefore();
+    reveal_EverySentIntraViewMsgIsForAViewLessOrEqualToSenderView();
+    reveal_EveryCommitClientOpMatchesRecordedPrePrepare();
+    h_v.workingWindow.reveal_Shift();
+  }
+
+  lemma HonestPreservesHonestReplicasLockOnPrepareForGivenView(c: Constants, v:Variables, v':Variables, step:Step, h_v:Replica.Variables, h_step:Replica.Step)
+    requires Inv(c, v)
+    requires HonestReplicaStepTaken(c, v, v', step, h_v, h_step)
+    ensures HonestReplicasLockOnPrepareForGivenView(c, v')
+  {
+    reveal_HonestReplicasLockOnPrepareForGivenView();
+    reveal_EveryPrepareClientOpMatchesRecordedPrePrepare();
+  }
+
+  lemma HonestPreservesHonestReplicasLockOnCommitForGivenView(c: Constants, v:Variables, v':Variables, step:Step, h_v:Replica.Variables, h_step:Replica.Step)
+    requires Inv(c, v)
+    requires HonestReplicaStepTaken(c, v, v', step, h_v, h_step)
+    ensures HonestReplicasLockOnCommitForGivenView(c, v')
+  {
+    reveal_HonestReplicasLockOnCommitForGivenView();
+    reveal_EveryCommitClientOpMatchesRecordedPrePrepare();
+  }
+
+  lemma HonestPreservesCommitMsgsFromHonestSendersAgree(c: Constants, v:Variables, v':Variables, step:Step, h_v:Replica.Variables, h_step:Replica.Step)
+    requires Inv(c, v)
+    requires HonestReplicaStepTaken(c, v, v', step, h_v, h_step)
     ensures CommitMsgsFromHonestSendersAgree(c, v')
   {
     reveal_CommitMsgsFromHonestSendersAgree();
@@ -485,41 +700,17 @@ module Proof {
       }
   }
 
-  lemma CommitMsgStability(c: Constants, v:Variables, v':Variables, step:Step)
+  lemma HonestPreservesRecordedCheckpointsRecvdCameFromNetwork(c: Constants, v:Variables, v':Variables, step:Step, h_v:Replica.Variables, h_step:Replica.Step)
     requires Inv(c, v)
-    requires NextStep(c, v, v', step)
-    ensures RecordedCommitsClientOpsMatchPrePrepare(c, v')
-    ensures EveryCommitIsSupportedByPreviouslySentPrepares(c, v')
-    ensures EveryPrepareClientOpMatchesRecordedPrePrepare(c, v')
-    ensures EveryCommitClientOpMatchesRecordedPrePrepare(c, v')
-    ensures HonestReplicasLockOnCommitForGivenView(c, v')
-    ensures EveryCommitMsgIsSupportedByAQuorumOfPrepares(c, v')
-    ensures CommitMsgsFromHonestSendersAgree(c, v')
+    requires HonestReplicaStepTaken(c, v, v', step, h_v, h_step)
+    ensures RecordedCheckpointsRecvdCameFromNetwork(c, v')
   {
-    ProofEveryCommitMsgIsSupportedByAQuorumOfPrepares(c, v, v', step);
-    reveal_RecordedCommitsClientOpsMatchPrePrepare();
-    reveal_EveryCommitIsSupportedByPreviouslySentPrepares();
-    reveal_EveryPrepareClientOpMatchesRecordedPrePrepare();
-    reveal_EveryCommitClientOpMatchesRecordedPrePrepare();
-    reveal_HonestReplicasLockOnCommitForGivenView();
-    ProofCommitMsgsFromHonestSendersAgree(c, v, v', step);
+    reveal_RecordedCheckpointsRecvdCameFromNetwork();
+    h_v.workingWindow.reveal_Shift();
   }
 
   lemma QuorumOfPreparesInNetworkMonotonic(c: Constants, v:Variables, v':Variables, step:Step)
     requires NextStep(c, v, v', step)
-    requires (c.clusterConfig.IsHonestReplica(step.id)
-              && var h_c := c.hosts[step.id].replicaConstants;
-                 var h_v := v.hosts[step.id].replicaVariables;
-                 var h_v' := v'.hosts[step.id].replicaVariables;
-                 var h_step :| Replica.NextStep(h_c, h_v, h_v', step.msgOps, h_step);
-                 Replica.NextStep(h_c, h_v, h_v', step.msgOps, h_step))
-              || 
-              (c.clusterConfig.IsFaultyReplica(step.id)
-               && var h_c := c.hosts[step.id].faultyReplicaConstants;
-                  var h_v := v.hosts[step.id].faultyReplicaVariables;
-                  var h_v' := v'.hosts[step.id].faultyReplicaVariables;
-                  var h_step :| FaultyReplica.NextStep(h_c, h_v, h_v', step.msgOps, h_step);
-                  FaultyReplica.NextStep(h_c, h_v, h_v', step.msgOps, h_step))
     ensures (forall view, seqID, clientOp | QuorumOfPreparesInNetwork(c, v, view, seqID, clientOp)
                                         :: QuorumOfPreparesInNetwork(c, v', view, seqID, clientOp))
   {
@@ -532,582 +723,97 @@ module Proof {
     }
   }
 
-  lemma ProofEveryCommitMsgIsSupportedByAQuorumOfPrepares(c: Constants, v:Variables, v':Variables, step:Step)
-    requires Inv(c, v)
-    requires NextStep(c, v, v', step)
-    ensures EveryCommitMsgIsSupportedByAQuorumOfPrepares(c, v')
-  {
-    // A proof of EveryCommitMsgIsSupportedByAQuorumOfPrepares,
-    // by selecting an arbitrary commitMsg instance
-    forall commitMsg | && commitMsg in v'.network.sentMsgs 
-                       && commitMsg.payload.Commit?
-                       && IsHonestReplica(c, commitMsg.sender) ensures 
-      QuorumOfPreparesInNetwork(c, v', commitMsg.payload.view, commitMsg.payload.seqID, commitMsg.payload.operationWrapper) {
-      if(commitMsg in v.network.sentMsgs) { // the commitMsg has been sent in a previous step
-        // In this case, the proof is trivial - we just need to "teach" Dafny about subset cardinality
-        var senders := Messages.sendersOf(sentPreparesForSeqID(c, v, commitMsg.payload.view, 
-                                                      commitMsg.payload.seqID, commitMsg.payload.operationWrapper));
-        var senders' := Messages.sendersOf(sentPreparesForSeqID(c, v', commitMsg.payload.view,
-                                                      commitMsg.payload.seqID, commitMsg.payload.operationWrapper));
-        Library.SubsetCardinality(senders, senders');
-      } else { // the commitMsg is being sent in the current step
-        var prepares := sentPreparesForSeqID(c, v, commitMsg.payload.view,
-                                             commitMsg.payload.seqID, commitMsg.payload.operationWrapper);
-        var prepares' := sentPreparesForSeqID(c, v', commitMsg.payload.view, 
-                                             commitMsg.payload.seqID, commitMsg.payload.operationWrapper);
-        assert prepares == prepares'; // Trigger (hint) - sending a commitMsg does not affect the set of prepares
-        
-        // Prove that the prepares in the working window are a subset of the prepares in the network:
-        var prepareSendersFromNetwork := Messages.sendersOf(prepares);
-        var h_v := v.hosts[step.id];
-        var prepareSendersInWorkingWindow := h_v.replicaVariables.workingWindow.preparesRcvd[commitMsg.payload.seqID].Keys;
-        assert (forall sender | sender in prepareSendersInWorkingWindow 
-                              :: && var msg := h_v.replicaVariables.workingWindow.preparesRcvd[commitMsg.payload.seqID][sender];
-                                 && msg in v.network.sentMsgs);
-        assert (forall sender | sender in prepareSendersInWorkingWindow 
-                              :: sender in prepareSendersFromNetwork); //Trigger for subset operator
-        Library.SubsetCardinality(prepareSendersInWorkingWindow, prepareSendersFromNetwork);
-      }
-    }
-  }
-
-  predicate SentCommitStepWasTaken(c: Constants, v:Variables, v':Variables,
-                                step:Step, h_step:Replica.Step)
-    requires Inv(c, v)
-  {
-    && NextStep(c, v, v', step)
-    && IsHonestReplica(c, step.id)
-    && var h_c := c.hosts[step.id].replicaConstants;
-    && var h_v := v.hosts[step.id].replicaVariables;
-    && var h_v' := v'.hosts[step.id].replicaVariables;
-    && Replica.NextStep(h_c, h_v, h_v', step.msgOps, h_step)
-    && h_step.SendCommitStep?
-    && Replica.SendCommit(h_c, h_v, h_v', step.msgOps, h_step.seqID)
-  }
-
-  lemma SendCommitStepPreservesInv(c: Constants, v:Variables, v':Variables, 
-                                   step:Step, h_step:Replica.Step)
-    requires Inv(c, v)
-    requires SentCommitStepWasTaken(c, v, v', step, h_step)
-    ensures Inv(c, v')
-  {
-    CommitMsgStability(c, v, v', step);
-  }
-
-  predicate SendClientOperationStepWasTaken(c: Constants, v:Variables, v':Variables,
-                                         step:Step, h_step:Client.Step)
-    requires Inv(c, v)
-  {
-    && NextStep(c, v, v', step)
-    && c.clusterConfig.IsClient(step.id)
-    && var h_c := c.hosts[step.id].clientConstants;
-    && var h_v := v.hosts[step.id].clientVariables;
-    && var h_v' := v'.hosts[step.id].clientVariables;
-    && Client.NextStep(h_c, h_v, h_v', step.msgOps, h_step)
-    && h_step.SendClientOperationStep?
-    && Client.SendClientOperation(h_c, h_v, h_v', step.msgOps)
-  }
-
-  lemma SendClientOperationPreservesInv(c: Constants, v:Variables, v':Variables, 
-                                   step:Step, h_step:Client.Step)
-    requires Inv(c, v)
-    requires SendClientOperationStepWasTaken(c, v, v', step, h_step)
-    ensures Inv(c, v')
-  {
-    CommitMsgStability(c, v, v', step);
-  }
-
-  predicate SendPrePrepareStepWasTaken(c: Constants, v:Variables, v':Variables,
-                                    step:Step, h_step:Replica.Step)
-    requires Inv(c, v)
-  {
-    && NextStep(c, v, v', step)
-    && IsHonestReplica(c, step.id)
-    && var h_c := c.hosts[step.id].replicaConstants;
-    && var h_v := v.hosts[step.id].replicaVariables;
-    && var h_v' := v'.hosts[step.id].replicaVariables;
-    && Replica.NextStep(h_c, h_v, h_v', step.msgOps, h_step)
-    && h_step.SendPrePrepareStep?
-    && Replica.SendPrePrepare(h_c, h_v, h_v', step.msgOps, h_step.seqID)
-  }
-
-  lemma SendPrePrepareStepPreservesInv(c: Constants, v:Variables, v':Variables, 
-                                       step:Step, h_step:Replica.Step)
-    requires Inv(c, v)
-    requires SendPrePrepareStepWasTaken(c, v, v', step, h_step)
-    ensures Inv(c, v')
-  {
-    CommitMsgStability(c, v, v', step);
-  }
-
-  predicate SendPrepareStepWasTaken(c: Constants, v:Variables, v':Variables,
-                                    step:Step, h_step:Replica.Step)
-    requires Inv(c, v)
-  {
-    && NextStep(c, v, v', step)
-    && IsHonestReplica(c, step.id)
-    && var h_c := c.hosts[step.id].replicaConstants;
-    && var h_v := v.hosts[step.id].replicaVariables;
-    && var h_v' := v'.hosts[step.id].replicaVariables;
-    && Replica.NextStep(h_c, h_v, h_v', step.msgOps, h_step)
-    && h_step.SendPrepareStep?
-    && Replica.SendPrepare(h_c, h_v, h_v', step.msgOps, h_step.seqID)
-  }
-
-  lemma SendPrepareStepPreservesInv(c: Constants, v:Variables, v':Variables, 
-                                       step:Step, h_step:Replica.Step)
-    requires Inv(c, v)
-    requires SendPrepareStepWasTaken(c, v, v', step, h_step)
-    ensures Inv(c, v')
-  {
-    reveal_EveryPrepareClientOpMatchesRecordedPrePrepare();
-    CommitMsgStability(c, v, v', step);
-  }
-
-  predicate RecvPrePrepareStepWasTaken(c: Constants, v:Variables, v':Variables,
-                                    step:Step, h_step:Replica.Step)
-    requires Inv(c, v)
-  {
-    && NextStep(c, v, v', step)
-    && IsHonestReplica(c, step.id)
-    && var h_c := c.hosts[step.id].replicaConstants;
-    && var h_v := v.hosts[step.id].replicaVariables;
-    && var h_v' := v'.hosts[step.id].replicaVariables;
-    && Replica.NextStep(h_c, h_v, h_v', step.msgOps, h_step)
-    && h_step.RecvPrePrepareStep?
-    && Replica.RecvPrePrepare(h_c, h_v, h_v', step.msgOps)
-  }
-
-  lemma RecvPrePrepareStepPreservesInv(c: Constants, v:Variables, v':Variables, 
-                                   step:Step, h_step:Replica.Step)
-    requires Inv(c, v)
-    requires RecvPrePrepareStepWasTaken(c, v, v', step, h_step)
-    ensures Inv(c, v')
-  {
-    CommitMsgStability(c, v, v', step);
-  }
-
-  predicate RecvPrepareStepWasTaken(c: Constants, v:Variables, v':Variables,
-                                step:Step, h_step:Replica.Step)
-    requires Inv(c, v)
-  {
-    && NextStep(c, v, v', step)
-    && IsHonestReplica(c, step.id)
-    && var h_c := c.hosts[step.id].replicaConstants;
-    && var h_v := v.hosts[step.id].replicaVariables;
-    && var h_v' := v'.hosts[step.id].replicaVariables;
-    && Replica.NextStep(h_c, h_v, h_v', step.msgOps, h_step)
-    && h_step.RecvPrepareStep?
-    && Replica.RecvPrepare(h_c, h_v, h_v', step.msgOps)
-  }
-
-  lemma RecvPrepareStepPreservesInv(c: Constants, v:Variables, v':Variables, 
-                                   step:Step, h_step:Replica.Step)
-    requires Inv(c, v)
-    requires RecvPrepareStepWasTaken(c, v, v', step, h_step)
-    ensures Inv(c, v')
-  {
-    CommitMsgStability(c, v, v', step);
-  }
-
-  predicate RecvCommitStepWasTaken(c: Constants, v:Variables, v':Variables,
-                                step:Step, h_step:Replica.Step)
-    requires Inv(c, v)
-  {
-    && NextStep(c, v, v', step)
-    && IsHonestReplica(c, step.id)
-    && var h_c := c.hosts[step.id].replicaConstants;
-    && var h_v := v.hosts[step.id].replicaVariables;
-    && var h_v' := v'.hosts[step.id].replicaVariables;
-    && Replica.NextStep(h_c, h_v, h_v', step.msgOps, h_step)
-    && h_step.RecvCommitStep?
-    && Replica.RecvCommit(h_c, h_v, h_v', step.msgOps)
-  }
-
-  lemma RecvCommitStepPreservesInv(c: Constants, v:Variables, v':Variables, 
-                                   step:Step, h_step:Replica.Step)
-    requires Inv(c, v)
-    requires RecvCommitStepWasTaken(c, v, v', step, h_step)
-    ensures Inv(c, v')
-  {
-    CommitMsgStability(c, v, v', step);
-  }
-
-  predicate DoCommitStepWasTaken(c: Constants, v:Variables, v':Variables,
-                                step:Step, h_step:Replica.Step)
-    requires Inv(c, v)
-  {
-    && NextStep(c, v, v', step)
-    && IsHonestReplica(c, step.id)
-    && var h_c := c.hosts[step.id].replicaConstants;
-    && var h_v := v.hosts[step.id].replicaVariables;
-    && var h_v' := v'.hosts[step.id].replicaVariables;
-    && Replica.NextStep(h_c, h_v, h_v', step.msgOps, h_step)
-    && h_step.DoCommitStep?
-    && Replica.DoCommit(h_c, h_v, h_v', step.msgOps, h_step.seqID)
-  }
-
-  lemma DoCommitStepPreservesInv(c: Constants, v:Variables, v':Variables, 
-                                   step:Step, h_step:Replica.Step)
-    requires Inv(c, v)
-    requires DoCommitStepWasTaken(c, v, v', step, h_step)
-    ensures Inv(c, v')
-  {
-    CommitMsgStability(c, v, v', step);
-  }
-
-  predicate ExecuteStepStepWasTaken(c: Constants, v:Variables, v':Variables,
-                                   step:Step, h_step:Replica.Step)
-    requires Inv(c, v)
-  {
-    && NextStep(c, v, v', step)
-    && IsHonestReplica(c, step.id)
-    && var h_c := c.hosts[step.id].replicaConstants;
-    && var h_v := v.hosts[step.id].replicaVariables;
-    && var h_v' := v'.hosts[step.id].replicaVariables;
-    && Replica.NextStep(h_c, h_v, h_v', step.msgOps, h_step)
-    && h_step.ExecuteStep?
-    && Replica.Execute(h_c, h_v, h_v', step.msgOps, h_step.seqID)
-  }
-
-  lemma ExecuteStepPreservesInv(c: Constants, v:Variables, v':Variables, 
-                                  step:Step, h_step:Replica.Step)
-    requires Inv(c, v)
-    requires ExecuteStepStepWasTaken(c, v, v', step, h_step)
-    ensures Inv(c, v')
-  {
-    CommitMsgStability(c, v, v', step);
-  }
-
-  predicate SendCheckpointStepStepWasTaken(c: Constants, v:Variables, v':Variables,
-                                   step:Step, h_step:Replica.Step)
-    requires Inv(c, v)
-  {
-    && NextStep(c, v, v', step)
-    && IsHonestReplica(c, step.id)
-    && var h_c := c.hosts[step.id].replicaConstants;
-    && var h_v := v.hosts[step.id].replicaVariables;
-    && var h_v' := v'.hosts[step.id].replicaVariables;
-    && Replica.NextStep(h_c, h_v, h_v', step.msgOps, h_step)
-    && h_step.SendCheckpointStep?
-    && Replica.SendCheckpoint(h_c, h_v, h_v', step.msgOps, h_step.seqID)
-  }
-
-  lemma SendCheckpointStepPreservesInv(c: Constants, v:Variables, v':Variables, 
-                                  step:Step, h_step:Replica.Step)
-    requires Inv(c, v)
-    requires SendCheckpointStepStepWasTaken(c, v, v', step, h_step)
-    ensures Inv(c, v')
-  {
-    CommitMsgStability(c, v, v', step);
-  }
-
-  predicate RecvCheckpointStepStepWasTaken(c: Constants, v:Variables, v':Variables,
-                                   step:Step, h_step:Replica.Step)
-    requires Inv(c, v)
-  {
-    && NextStep(c, v, v', step)
-    && IsHonestReplica(c, step.id)
-    && var h_c := c.hosts[step.id].replicaConstants;
-    && var h_v := v.hosts[step.id].replicaVariables;
-    && var h_v' := v'.hosts[step.id].replicaVariables;
-    && Replica.NextStep(h_c, h_v, h_v', step.msgOps, h_step)
-    && h_step.RecvCheckpointStep?
-    && Replica.RecvCheckpoint(h_c, h_v, h_v', step.msgOps)
-  }
-
-  lemma RecvCheckpointStepPreservesInv(c: Constants, v:Variables, v':Variables, 
-                                  step:Step, h_step:Replica.Step)
-    requires Inv(c, v)
-    requires RecvCheckpointStepStepWasTaken(c, v, v', step, h_step)
-    ensures Inv(c, v')
-  {
-    CommitMsgStability(c, v, v', step);
-  }
-  predicate AdvanceWorkingWindowStepStepWasTaken(c: Constants, v:Variables, v':Variables,
-                                   step:Step, h_step:Replica.Step)
-    requires Inv(c, v)
-  {
-    && NextStep(c, v, v', step)
-    && IsHonestReplica(c, step.id)
-    && var h_c := c.hosts[step.id].replicaConstants;
-    && var h_v := v.hosts[step.id].replicaVariables;
-    && var h_v' := v'.hosts[step.id].replicaVariables;
-    && Replica.NextStep(h_c, h_v, h_v', step.msgOps, h_step)
-    && h_step.AdvanceWorkingWindowStep?
-    && Replica.AdvanceWorkingWindow(h_c, h_v, h_v', step.msgOps, h_step.seqID, h_step.checkpointsQuorum)
-  }
-
-  lemma AdvanceWorkingWindowStepPreservesInv(c: Constants, v:Variables, v':Variables, 
-                                  step:Step, h_step:Replica.Step)
-    requires Inv(c, v)
-    requires AdvanceWorkingWindowStepStepWasTaken(c, v, v', step, h_step)
-    ensures Inv(c, v')
-  {
-    CommitMsgStability(c, v, v', step);
-  }
-
-  predicate PerformStateTransferStepStepWasTaken(c: Constants, v:Variables, v':Variables,
-                                   step:Step, h_step:Replica.Step)
-    requires Inv(c, v)
-  {
-    && NextStep(c, v, v', step)
-    && IsHonestReplica(c, step.id)
-    && var h_c := c.hosts[step.id].replicaConstants;
-    && var h_v := v.hosts[step.id].replicaVariables;
-    && var h_v' := v'.hosts[step.id].replicaVariables;
-    && Replica.NextStep(h_c, h_v, h_v', step.msgOps, h_step)
-    && h_step.PerformStateTransferStep?
-    && Replica.PerformStateTransfer(h_c, h_v, h_v', step.msgOps, h_step.seqID, h_step.checkpointsQuorum)
-  }
-
-  lemma PerformStateTransferStepPreservesInv(c: Constants, v:Variables, v':Variables, 
-                                  step:Step, h_step:Replica.Step)
-    requires Inv(c, v)
-    requires PerformStateTransferStepStepWasTaken(c, v, v', step, h_step)
-    ensures Inv(c, v')
-  {
-    CommitMsgStability(c, v, v', step);
-  }
-
-  predicate LeaveViewStepStepWasTaken(c: Constants, v:Variables, v':Variables,
-                                   step:Step, h_step:Replica.Step)
-    requires Inv(c, v)
-  {
-    && NextStep(c, v, v', step)
-    && IsHonestReplica(c, step.id)
-    && var h_c := c.hosts[step.id].replicaConstants;
-    && var h_v := v.hosts[step.id].replicaVariables;
-    && var h_v' := v'.hosts[step.id].replicaVariables;
-    && Replica.NextStep(h_c, h_v, h_v', step.msgOps, h_step)
-    && h_step.LeaveViewStep?
-    && Replica.LeaveView(h_c, h_v, h_v', step.msgOps, h_step.newView)
-  }
-
-  lemma LeaveViewStepPreservesInv(c: Constants, v:Variables, v':Variables, 
-                                  step:Step, h_step:Replica.Step)
-    requires Inv(c, v)
-    requires LeaveViewStepStepWasTaken(c, v, v', step, h_step)
-    ensures Inv(c, v')
-  {
-    CommitMsgStability(c, v, v', step);
-  }
-
-  predicate SendViewChangeMsgStepStepWasTaken(c: Constants, v:Variables, v':Variables,
-                                   step:Step, h_step:Replica.Step)
-    requires Inv(c, v)
-  {
-    && NextStep(c, v, v', step)
-    && IsHonestReplica(c, step.id)
-    && var h_c := c.hosts[step.id].replicaConstants;
-    && var h_v := v.hosts[step.id].replicaVariables;
-    && var h_v' := v'.hosts[step.id].replicaVariables;
-    && Replica.NextStep(h_c, h_v, h_v', step.msgOps, h_step)
-    && h_step.SendViewChangeMsgStep?
-    && Replica.SendViewChangeMsg(h_c, h_v, h_v', step.msgOps)
-  }
-
-  lemma SendViewChangeMsgStepPreservesInv(c: Constants, v:Variables, v':Variables, 
-                                  step:Step, h_step:Replica.Step)
-    requires Inv(c, v)
-    requires SendViewChangeMsgStepStepWasTaken(c, v, v', step, h_step)
-    ensures Inv(c, v')
-  {
-    CommitMsgStability(c, v, v', step);
-  }
-
-  predicate RecvViewChangeMsgStepStepWasTaken(c: Constants, v:Variables, v':Variables,
-                                   step:Step, h_step:Replica.Step)
-    requires Inv(c, v)
-  {
-    && NextStep(c, v, v', step)
-    && IsHonestReplica(c, step.id)
-    && var h_c := c.hosts[step.id].replicaConstants;
-    && var h_v := v.hosts[step.id].replicaVariables;
-    && var h_v' := v'.hosts[step.id].replicaVariables;
-    && Replica.NextStep(h_c, h_v, h_v', step.msgOps, h_step)
-    && h_step.RecvViewChangeMsgStep?
-    && Replica.RecvViewChangeMsg(h_c, h_v, h_v', step.msgOps)
-  }
-
-  lemma RecvViewChangeMsgStepPreservesInv(c: Constants, v:Variables, v':Variables, 
-                                  step:Step, h_step:Replica.Step)
-    requires Inv(c, v)
-    requires RecvViewChangeMsgStepStepWasTaken(c, v, v', step, h_step)
-    ensures Inv(c, v')
-  {
-    CommitMsgStability(c, v, v', step);
-  }
-
-  predicate SelectQuorumOfViewChangeMsgsStepStepWasTaken(c: Constants, v:Variables, v':Variables,
-                                   step:Step, h_step:Replica.Step)
-    requires Inv(c, v)
-  {
-    && NextStep(c, v, v', step)
-    && IsHonestReplica(c, step.id)
-    && var h_c := c.hosts[step.id].replicaConstants;
-    && var h_v := v.hosts[step.id].replicaVariables;
-    && var h_v' := v'.hosts[step.id].replicaVariables;
-    && Replica.NextStep(h_c, h_v, h_v', step.msgOps, h_step)
-    && h_step.SelectQuorumOfViewChangeMsgsStep?
-    && Replica.SelectQuorumOfViewChangeMsgs(h_c, h_v, h_v', step.msgOps, h_step.viewChangeMsgsSelectedByPrimary)
-  }
-
-  lemma SelectQuorumOfViewChangeMsgsStepPreservesInv(c: Constants, v:Variables, v':Variables, 
-                                  step:Step, h_step:Replica.Step)
-    requires Inv(c, v)
-    requires SelectQuorumOfViewChangeMsgsStepStepWasTaken(c, v, v', step, h_step)
-    ensures Inv(c, v')
-  {
-    CommitMsgStability(c, v, v', step);
-  }
-
-  predicate SendNewViewMsgStepStepWasTaken(c: Constants, v:Variables, v':Variables,
-                                   step:Step, h_step:Replica.Step)
-    requires Inv(c, v)
-  {
-    && NextStep(c, v, v', step)
-    && IsHonestReplica(c, step.id)
-    && var h_c := c.hosts[step.id].replicaConstants;
-    && var h_v := v.hosts[step.id].replicaVariables;
-    && var h_v' := v'.hosts[step.id].replicaVariables;
-    && Replica.NextStep(h_c, h_v, h_v', step.msgOps, h_step)
-    && h_step.SendNewViewMsgStep?
-    && Replica.SendNewViewMsg(h_c, h_v, h_v', step.msgOps)
-  }
-
-  lemma SendNewViewMsgStepPreservesInv(c: Constants, v:Variables, v':Variables, 
-                                  step:Step, h_step:Replica.Step)
-    requires Inv(c, v)
-    requires SendNewViewMsgStepStepWasTaken(c, v, v', step, h_step)
-    ensures Inv(c, v')
-  {
-    CommitMsgStability(c, v, v', step);
-  }
-
-  predicate RecvNewViewMsgStepStepWasTaken(c: Constants, v:Variables, v':Variables,
-                                   step:Step, h_step:Replica.Step)
-    requires Inv(c, v)
-  {
-    && NextStep(c, v, v', step)
-    && IsHonestReplica(c, step.id)
-    && var h_c := c.hosts[step.id].replicaConstants;
-    && var h_v := v.hosts[step.id].replicaVariables;
-    && var h_v' := v'.hosts[step.id].replicaVariables;
-    && Replica.NextStep(h_c, h_v, h_v', step.msgOps, h_step)
-    && h_step.RecvNewViewMsgStep?
-    && Replica.RecvNewViewMsg(h_c, h_v, h_v', step.msgOps)
-  }
-
-  lemma RecvNewViewMsgStepPreservesInv(c: Constants, v:Variables, v':Variables, 
-                                  step:Step, h_step:Replica.Step)
-    requires Inv(c, v)
-    requires RecvNewViewMsgStepStepWasTaken(c, v, v', step, h_step)
-    ensures Inv(c, v')
-  {
-    CommitMsgStability(c, v, v', step);
-  }
-
   lemma InvariantNext(c: Constants, v:Variables, v':Variables)
     requires Inv(c, v)
     requires Next(c, v, v')
     ensures Inv(c, v')
   {
     var step :| NextStep(c, v, v', step);
-
-    if (c.clusterConfig.IsHonestReplica(step.id))
-    {
+    if IsHonestReplica(c, step.id) {
       var h_c := c.hosts[step.id].replicaConstants;
       var h_v := v.hosts[step.id].replicaVariables;
       var h_v' := v'.hosts[step.id].replicaVariables;
       var h_step :| Replica.NextStep(h_c, h_v, h_v', step.msgOps, h_step);
-      
-      //QuorumOfPreparesInNetworkMonotonic(c, v, v', step, h_step); // not part of the proof yet
-      
-      match h_step
-        case SendPrePrepareStep(seqID) => {
-          SendPrePrepareStepPreservesInv(c, v, v', step, h_step);
-        }
-        case RecvPrePrepareStep() => {
-          RecvPrePrepareStepPreservesInv(c, v, v', step, h_step);
-        }
-        case SendPrepareStep(seqID) => {
-          SendPrepareStepPreservesInv(c, v, v', step, h_step);
-        }
-        case RecvPrepareStep() => { 
-          RecvPrepareStepPreservesInv(c, v, v', step, h_step);
-        }
-        case SendCommitStep(seqID) => {
-          SendCommitStepPreservesInv(c, v, v', step, h_step);
-        }
-        case RecvCommitStep() => {
-          RecvCommitStepPreservesInv(c, v, v', step, h_step);
-        }
-        case DoCommitStep(seqID) => { 
-          DoCommitStepPreservesInv(c, v, v', step, h_step);
-        }
-        case ExecuteStep(seqID) => {
-          ExecuteStepPreservesInv(c, v, v', step, h_step);
-        }
-        case SendCheckpointStep(seqID) => {
-          SendCheckpointStepPreservesInv(c, v, v', step, h_step);
-        }
-        case RecvCheckpointStep() => {
-          RecvCheckpointStepPreservesInv(c, v, v', step, h_step);
-        }
-        case AdvanceWorkingWindowStep(seqID, checkpointsQuorum) => {
-          AdvanceWorkingWindowStepPreservesInv(c, v, v', step, h_step);
-        }
-        case PerformStateTransferStep(seqID, checkpointsQuorum) => {
-          PerformStateTransferStepPreservesInv(c, v, v', step, h_step);
-        }
-        case LeaveViewStep(newView) => {
-          LeaveViewStepPreservesInv(c, v, v', step, h_step);
-        }
-        case SendViewChangeMsgStep() => {
-          SendViewChangeMsgStepPreservesInv(c, v, v', step, h_step);
-        }
-        case RecvViewChangeMsgStep() => {
-          RecvViewChangeMsgStepPreservesInv(c, v, v', step, h_step);
-        }
-        case SelectQuorumOfViewChangeMsgsStep(viewChangeMsgsSelectedByPrimary) => {
-          SelectQuorumOfViewChangeMsgsStepPreservesInv(c, v, v', step, h_step);
-        }
-        case SendNewViewMsgStep() => {
-          SendNewViewMsgStepPreservesInv(c, v, v', step, h_step);
-        }
-        case RecvNewViewMsgStep() => {
-          RecvNewViewMsgStepPreservesInv(c, v, v', step, h_step);
-        }
-
-    } else if (c.clusterConfig.IsClient(step.id)) {
-
-      var h_c := c.hosts[step.id].clientConstants;
-      var h_v := v.hosts[step.id].clientVariables;
-      var h_v' := v'.hosts[step.id].clientVariables;
-      var h_step :| Client.NextStep(h_c, h_v, h_v', step.msgOps, h_step);
-
-      match h_step
-        case SendClientOperationStep() => {
-          SendClientOperationPreservesInv(c, v, v', step, h_step);
-        }
-    } else if(c.clusterConfig.IsFaultyReplica(step.id)) {
-      InvNextFaulty(c, v, v', step);
-      CommitMsgStability(c, v, v', step);
+      assert HonestReplicaStepTaken(c, v, v', step, h_v, h_step);
+      HonestPreservesAllReplicasLiteInv(c, v, v', step, h_v, h_step);
+      HonestPreservesRecordedPreparesHaveValidSenderID(c, v, v', step, h_v, h_step);
+      HonestPreservesRecordedPrePreparesRecvdCameFromNetwork(c, v, v', step, h_v, h_step);
+      HonestPreservesRecordedPreparesInAllHostsRecvdCameFromNetwork(c, v, v', step, h_v, h_step);
+      HonestPreservesRecordedPreparesMatchHostView(c, v, v', step, h_v, h_step);
+      AlwaysPreservesEveryCommitMsgIsSupportedByAQuorumOfPrepares(c, v, v', step);
+      HonestPreservesRecordedPreparesClientOpsMatchPrePrepare(c, v, v', step, h_v, h_step);
+      HonestPreservesRecordedCommitsClientOpsMatchPrePrepare(c, v, v', step, h_v, h_step);
+      HonestPreservesEverySentIntraViewMsgIsInWorkingWindowOrBefore(c, v, v', step, h_v, h_step);
+      HonestPreservesEverySentIntraViewMsgIsForAViewLessOrEqualToSenderView(c, v, v', step, h_v, h_step);
+      HonestPreservesEveryPrepareClientOpMatchesRecordedPrePrepare(c, v, v', step, h_v, h_step);
+      HonestPreservesEveryCommitClientOpMatchesRecordedPrePrepare(c, v, v', step, h_v, h_step);
+      HonestPreservesHonestReplicasLockOnPrepareForGivenView(c, v, v', step, h_v, h_step);
+      HonestPreservesHonestReplicasLockOnCommitForGivenView(c, v, v', step, h_v, h_step);
+      HonestPreservesCommitMsgsFromHonestSendersAgree(c, v, v', step, h_v, h_step);
+      HonestPreservesRecordedCheckpointsRecvdCameFromNetwork(c, v, v', step, h_v, h_step);
     } else {
-      assert false; // Should not be possible
+      InvNextFaultyOrClient(c, v, v', step);
     }
   }
 
-  lemma InvNextFaulty(c: Constants, v:Variables, v':Variables, step: Step)
+  lemma InvNextFaultyOrClient(c: Constants, v:Variables, v':Variables, step: Step)
     requires v.WF(c)
-    requires c.clusterConfig.IsFaultyReplica(step.id)
-    requires HonestReplicasLockOnCommitForGivenView(c, v)
+    requires Inv(c, v)
     requires NextStep(c, v, v', step)
-    ensures HonestReplicasLockOnCommitForGivenView(c, v')
+    requires (c.clusterConfig.IsFaultyReplica(step.id) || c.clusterConfig.IsClient(step.id))
+    ensures Inv(c, v')
   {
-    reveal_HonestReplicasLockOnCommitForGivenView();
-    assert forall msg | msg in v'.network.sentMsgs && IsHonestReplica(c, msg.sender) :: msg in v.network.sentMsgs;
+    assert AllReplicasLiteInv(c, v') by {
+      reveal_AllReplicasLiteInv();
+    }
+    assert RecordedPreparesHaveValidSenderID(c, v') by {
+      reveal_RecordedPreparesHaveValidSenderID();
+    }
+    assert RecordedPrePreparesRecvdCameFromNetwork(c, v') by {
+      reveal_RecordedPrePreparesRecvdCameFromNetwork();
+    }
+    assert RecordedPreparesInAllHostsRecvdCameFromNetwork(c, v') by {
+      reveal_RecordedPreparesInAllHostsRecvdCameFromNetwork();
+    }
+    assert RecordedPreparesMatchHostView(c, v') by {
+      reveal_RecordedPreparesMatchHostView();
+    }
+    assert RecordedPreparesClientOpsMatchPrePrepare(c, v') by {
+      reveal_RecordedPreparesClientOpsMatchPrePrepare();
+    }
+    assert RecordedCommitsClientOpsMatchPrePrepare(c, v') by {
+      reveal_RecordedCommitsClientOpsMatchPrePrepare();
+    }
+    assert EverySentIntraViewMsgIsInWorkingWindowOrBefore(c, v') by {
+      reveal_EverySentIntraViewMsgIsInWorkingWindowOrBefore();
+    }
+    assert EverySentIntraViewMsgIsForAViewLessOrEqualToSenderView(c, v') by {
+      reveal_EverySentIntraViewMsgIsForAViewLessOrEqualToSenderView();
+    }
+    assert EveryPrepareClientOpMatchesRecordedPrePrepare(c, v') by {
+      reveal_EveryPrepareClientOpMatchesRecordedPrePrepare();
+    }
+    assert EveryCommitClientOpMatchesRecordedPrePrepare(c, v') by {
+      reveal_EveryCommitClientOpMatchesRecordedPrePrepare();
+    }
+    assert HonestReplicasLockOnPrepareForGivenView(c, v') by {
+      reveal_HonestReplicasLockOnPrepareForGivenView();
+    }
+    assert HonestReplicasLockOnCommitForGivenView(c, v') by {
+      reveal_HonestReplicasLockOnCommitForGivenView();
+    }
+    assert CommitMsgsFromHonestSendersAgree(c, v') by {
+      reveal_CommitMsgsFromHonestSendersAgree();
+    }
+    assert RecordedCheckpointsRecvdCameFromNetwork(c, v') by {
+      reveal_RecordedCheckpointsRecvdCameFromNetwork();
+    }
+    assert HonestReplicasLockOnCommitForGivenView(c, v') by {
+      reveal_HonestReplicasLockOnCommitForGivenView();
+    }
+    assert EveryCommitMsgIsSupportedByAQuorumOfPrepares(c, v') by {
+      AlwaysPreservesEveryCommitMsgIsSupportedByAQuorumOfPrepares(c, v, v', step);
+    }
   }
 
   lemma InvariantInductive(c: Constants, v:Variables, v':Variables)
@@ -1116,16 +822,27 @@ module Proof {
     //ensures Inv(c, v) ==> Safety(c, v)
   {
     if Init(c, v) {
-      reveal_RecordedCommitsClientOpsMatchPrePrepare();
-      reveal_EveryCommitIsSupportedByPreviouslySentPrepares();
-      reveal_EveryPrepareClientOpMatchesRecordedPrePrepare();
-      reveal_EveryCommitClientOpMatchesRecordedPrePrepare();
-      reveal_HonestReplicasLockOnCommitForGivenView();
-      reveal_CommitMsgsFromHonestSendersAgree();
-      assert Inv(c, v);
+      assert Inv(c, v) by {
+        reveal_AllReplicasLiteInv();
+        reveal_RecordedCommitsClientOpsMatchPrePrepare();
+        reveal_EveryPrepareClientOpMatchesRecordedPrePrepare();
+        reveal_EveryCommitClientOpMatchesRecordedPrePrepare();
+        reveal_HonestReplicasLockOnCommitForGivenView();
+        reveal_CommitMsgsFromHonestSendersAgree();
+        reveal_RecordedPreparesHaveValidSenderID();
+        reveal_RecordedPrePreparesRecvdCameFromNetwork();
+        reveal_RecordedPreparesInAllHostsRecvdCameFromNetwork();
+        reveal_RecordedPreparesMatchHostView();
+        reveal_RecordedPreparesClientOpsMatchPrePrepare();
+        reveal_EverySentIntraViewMsgIsInWorkingWindowOrBefore();
+        reveal_EverySentIntraViewMsgIsForAViewLessOrEqualToSenderView();
+        reveal_HonestReplicasLockOnPrepareForGivenView();
+        reveal_RecordedCheckpointsRecvdCameFromNetwork();
+        reveal_EveryCommitMsgIsSupportedByAQuorumOfPrepares();      
+      }
     }
     if Inv(c, v) && Next(c, v, v') {
       InvariantNext(c, v, v');
     }
   }
-}
+} //Module
